wip

systems/chord-props/QueryTargetsJoined.v
@@ -167,6 +167,584 @@ Proof.
 Admitted.
 *)
 
+Definition pointers_in_payload (sender : addr) (m : payload) :=
+  match m with
+  | GotPredAndSuccs (Some s) succs =>
+    make_pointer sender :: s :: succs
+  | GotPredAndSuccs None succs => make_pointer sender :: succs
+  | GotSuccList succs => make_pointer sender :: succs
+  | GotBestPredecessor s => [make_pointer sender; s]
+  | _ => []
+  end.
+
+Definition pointers_in_network gst :=
+  flat_map (fun m => pointers_in_payload (fst m) (snd (snd m))) (msgs gst).
+
+Definition option_to_list {A} (x : option A) :=
+  match x with
+  | None => []
+  | Some a => [a]
+  end.
+
+
+Definition pointers_in_node_state st :=
+  (option_to_list (pred st)) ++ (option_to_list (rectify_with st)) ++ succ_list st.
+
+Definition pointers_in_state gst :=
+  concat (filterMap (fun h => option_map pointers_in_node_state (sigma gst h)) (nodes gst))
+         ++ pointers_in_network gst.
+
+Definition concat_in :
+  forall A (l : list A) l' a,
+    In a l ->
+    In l l' ->
+    In a (concat l').
+Proof.
+  induction l'; in_crush.
+Qed.
+
+Definition in_succ_list_in_pointers_in_node_state :
+  forall st p,
+    In p (succ_list st) ->
+    In p (pointers_in_node_state st).
+Proof.
+  intros. unfold pointers_in_node_state.
+  in_crush.
+Qed.
+
+Lemma in_succ_list_in_pointers_in_state :
+  forall gst h st p,
+    In h (nodes gst) ->
+    sigma gst h = Some st ->
+    In p (succ_list st) ->
+    In p (pointers_in_state gst).
+Proof.
+  intros. unfold pointers_in_state.
+  find_apply_lem_hyp in_succ_list_in_pointers_in_node_state.
+  in_crush. left.
+  eapply concat_in; eauto.
+  eapply filterMap_In; eauto.
+  find_rewrite. reflexivity.
+Qed.
+
+Hint Resolve in_succ_list_in_pointers_in_state.
+
+Definition pred_in_pointers_in_node_state :
+  forall st p,
+    pred st = Some p ->
+    In p (pointers_in_node_state st).
+Proof.
+  intros. unfold pointers_in_node_state.
+  find_rewrite.
+  in_crush.
+Qed.
+
+Lemma pred_in_pointers_in_state :
+  forall gst h st p,
+    In h (nodes gst) ->
+    sigma gst h = Some st ->
+    pred st = Some p ->
+    In p (pointers_in_state gst).
+Proof.
+  intros. unfold pointers_in_state.
+  find_apply_lem_hyp pred_in_pointers_in_node_state.
+  in_crush. left.
+  eapply concat_in; eauto.
+  eapply filterMap_In; eauto.
+  find_rewrite. reflexivity.
+Qed.
+
+Hint Resolve pred_in_pointers_in_state.
+
+Definition rectify_with_in_pointers_in_node_state :
+  forall st p,
+    rectify_with st = Some p ->
+    In p (pointers_in_node_state st).
+Proof.
+  intros. unfold pointers_in_node_state.
+  find_rewrite.
+  in_crush.
+Qed.
+
+Lemma rectify_with_in_pointers_in_state :
+  forall gst h st p,
+    In h (nodes gst) ->
+    sigma gst h = Some st ->
+    rectify_with st = Some p ->
+    In p (pointers_in_state gst).
+Proof.
+  intros. unfold pointers_in_state.
+  find_apply_lem_hyp rectify_with_in_pointers_in_node_state.
+  in_crush. left.
+  eapply concat_in; eauto.
+  eapply filterMap_In; eauto.
+  find_rewrite. reflexivity.
+Qed.
+
+Hint Resolve rectify_with_in_pointers_in_state.
+
+Lemma in_network_in_pointers_in_state :
+  forall gst m p,
+    In m (msgs gst) ->
+    In p (pointers_in_payload (fst m) (snd (snd m))) ->
+    In p (pointers_in_state gst).
+Proof.
+  intros. unfold pointers_in_state.
+  in_crush. right. unfold pointers_in_network.
+  apply in_flat_map. eauto.
+Qed.
+
+Hint Resolve in_network_in_pointers_in_state.
+
+Lemma in_got_succ_list_in_pointers_in_state :
+  forall gst m p l,
+    In m (msgs gst) ->
+    snd (snd m) = GotSuccList l ->
+    In p l ->
+    In p (pointers_in_state gst).
+Proof.
+  intros. unfold pointers_in_state. in_crush.
+  right. unfold pointers_in_network. apply in_flat_map.
+  exists m. intuition; repeat find_rewrite; simpl; auto.
+Qed.
+
+Hint Resolve in_got_succ_list_in_pointers_in_state.
+
+
+Lemma sender_got_succ_list_in_pointers_in_state :
+  forall gst m l,
+    In m (msgs gst) ->
+    snd (snd m) = GotSuccList l ->
+    In (make_pointer (fst m)) (pointers_in_state gst).
+Proof.
+  intros. unfold pointers_in_state. in_crush.
+  right. unfold pointers_in_network. apply in_flat_map.
+  exists m. intuition; repeat find_rewrite; simpl; auto.
+Qed.
+
+Hint Resolve sender_got_succ_list_in_pointers_in_state.
+
+
+Lemma in_got_best_pred_in_pointers_in_state :
+  forall gst m p,
+    In m (msgs gst) ->
+    snd (snd m) = GotBestPredecessor p ->
+    In p (pointers_in_state gst).
+Proof.
+  intros. unfold pointers_in_state. in_crush.
+  right. unfold pointers_in_network. apply in_flat_map.
+  exists m. intuition; repeat find_rewrite; simpl; auto.
+Qed.
+
+Hint Resolve in_got_best_pred_in_pointers_in_state.
+
+
+Lemma sender_got_best_pred_in_pointers_in_state :
+  forall gst m p,
+    In m (msgs gst) ->
+    snd (snd m) = GotBestPredecessor p ->
+    In (make_pointer (fst m)) (pointers_in_state gst).
+Proof.
+  intros. unfold pointers_in_state. in_crush.
+  right. unfold pointers_in_network. apply in_flat_map.
+  exists m. intuition; repeat find_rewrite; simpl; auto.
+Qed.
+
+Hint Resolve sender_got_best_pred_in_pointers_in_state.
+
+
+Lemma filterMap_in :
+  forall A B (f : A -> option B) l x,
+    In x (filterMap f l) ->
+    exists y,
+      In y l /\
+      f y = Some x.
+Proof.
+  induction l; intros; in_crush.
+  break_match; in_crush; eauto;
+    eapply_prop_hyp @filterMap @filterMap;
+    break_exists_exists; intuition.
+Qed.
+
+Lemma in_option_to_list :
+  forall A (o : option A) x,
+    In x (option_to_list o) ->
+    o = Some x.
+Proof.
+  intros. unfold option_to_list in *.
+  break_match; in_crush.
+Qed.
+
+Lemma pointers_in_state_elim :
+  forall p gst,
+    In p (pointers_in_state gst) ->
+    (exists h st, In h (nodes gst) /\ sigma gst h = Some st /\ In p (succ_list st)) \/
+    (exists h st, In h (nodes gst) /\ sigma gst h = Some st /\ pred st = Some p) \/
+    (exists h st, In h (nodes gst) /\ sigma gst h = Some st /\ rectify_with st = Some p) \/
+    (exists m, In m (msgs gst) /\ In p (pointers_in_payload (fst m) (snd (snd m)))).
+Proof.
+  intros. unfold pointers_in_state in *.
+  in_crush.
+  - find_apply_lem_hyp in_concat.
+    break_exists. intuition.
+    find_apply_lem_hyp filterMap_in.
+    break_exists. intuition.
+    find_apply_lem_hyp option_map_Some.
+    break_exists.
+    intuition.
+    unfold pointers_in_node_state in *.
+    subst. in_crush.
+    + right. left. find_apply_lem_hyp in_option_to_list. eauto.
+    + right. right. left. find_apply_lem_hyp in_option_to_list. eauto.
+    + left. eauto.
+  - repeat right.
+    unfold pointers_in_network in *.
+    find_apply_lem_hyp in_flat_map.
+    eauto.
+Qed.
+
+Lemma check :
+  forall gst p,
+    In p (pointers_in_state gst) ->
+    In p (pointers_in_state gst).
+Proof.
+  intros. find_apply_lem_hyp pointers_in_state_elim.
+  intuition; break_exists; intuition eauto.
+Qed.
+
+Definition pointer_joined gst p :=
+  In (addr_of p) (nodes gst) /\
+  exists st,
+    sigma gst (addr_of p) = Some st /\
+    joined st = true.
+
+Lemma pointer_joined_stable :
+  forall gst gst' p,
+    reachable_st gst ->
+    step_dynamic gst gst' ->
+    pointer_joined gst p ->
+    pointer_joined gst' p.
+Proof.
+  intros. unfold pointer_joined in *. inv_prop step_dynamic; intuition.
+  - unfold update_for_start. simpl. intuition.
+  - unfold update_for_start. simpl. update_destruct; subst; rewrite_update; intuition.
+  - break_exists. intuition.
+    find_apply_lem_hyp timeout_handler_definition.
+    break_exists.
+    find_apply_lem_hyp joined_preserved_by_timeout_handler_eff.
+    unfold apply_handler_result. simpl.
+    update_destruct; subst; rewrite_update; intuition eauto.
+    eexists; intuition eauto. congruence.
+  - break_exists. intuition.
+    unfold apply_handler_result. simpl.
+    update_destruct; subst; rewrite_update; intuition eauto.
+    find_apply_lem_hyp joined_preserved_by_recv_handler; eauto.
+    congruence.
+Qed.
+
+Lemma find_pred_in :
+  forall h p l,
+    find_pred h l = Some p ->
+    In p l.
+Proof.
+  induction l using List.rev_ind.
+  - unfold find_pred. simpl. intuition. congruence.
+  - unfold find_pred. simpl.
+    rewrite rev_unit. simpl.
+    in_crush. find_inversion. auto.
+Qed.
+
+
+Lemma in_make_succs :
+  forall p s l,
+    In p (make_succs s l) ->
+    p = s \/ In p l.
+Proof.
+  unfold make_succs. intros.
+  find_apply_lem_hyp in_firstn.
+  in_crush.
+Qed.
+
+Lemma in_partition :
+  forall A (l : list A) xs a ys,
+    l = xs ++ a :: ys ->
+    In a l.
+Proof.
+  intros. in_crush.
+Qed.
+
+Hint Resolve in_partition.
+
+Theorem big_joined_invariant :
+  forall gst p,
+    reachable_st gst ->
+    In p (pointers_in_state gst) ->
+    pointer_joined gst p.
+Proof.
+  intros. induction H.
+  - find_apply_lem_hyp pointers_in_state_elim;
+    intuition; break_exists; intuition.
+    + find_copy_apply_lem_hyp sigma_initial_st_start_handler; eauto.
+      subst. unfold start_handler in *.
+      repeat break_match; simpl in *; intuition.
+      cut (In (addr_of p) (nodes gst)).
+      { intros. find_apply_lem_hyp initial_nodes_live; eauto.
+        unfold live_node in *. intuition. unfold pointer_joined; eauto.
+      }
+      cut (In p (sort_by_between x (map make_pointer (nodes gst)))).
+      {
+        intros.
+        find_apply_lem_hyp in_sort_by_between.
+        in_crush.
+      }
+      repeat find_rewrite.
+      find_apply_lem_hyp in_firstn.
+      in_crush.
+    + find_copy_apply_lem_hyp sigma_initial_st_start_handler; eauto.
+      subst. unfold start_handler in *.
+      repeat break_match; simpl in *; intuition; try congruence.
+      find_apply_lem_hyp find_pred_in.
+      cut (In (addr_of p) (nodes gst)).
+      { intros. find_apply_lem_hyp initial_nodes_live; eauto.
+        unfold live_node in *. intuition. unfold pointer_joined; eauto.
+      }
+      cut (In p (sort_by_between x (map make_pointer (nodes gst)))).
+      {
+        intros.
+        find_apply_lem_hyp in_sort_by_between.
+        in_crush.
+      }
+      repeat find_rewrite. auto.
+    + find_copy_apply_lem_hyp sigma_initial_st_start_handler; eauto.
+      subst. unfold start_handler in *.
+      repeat break_match; simpl in *; intuition; congruence.
+    + unfold initial_st in *. intuition. repeat find_rewrite. in_crush.
+  - assert (In p (pointers_in_state gst) -> pointer_joined gst' p) by
+        eauto using pointer_joined_stable.
+    inv_prop step_dynamic.
+    + find_apply_lem_hyp pointers_in_state_elim.
+      intuition; break_exists; intuition; simpl in *; eauto.
+      * update_destruct; subst; rewrite_update; intuition; subst; eauto.
+        find_inversion. simpl in *. intuition; congruence.
+      * update_destruct; subst; rewrite_update; intuition; subst; eauto.
+        find_inversion. simpl in *. intuition; congruence.
+      * update_destruct; subst; rewrite_update; intuition; subst; eauto.
+        find_inversion. simpl in *. intuition; congruence.
+      * intuition; eauto.
+        subst. simpl in *. intuition.
+    + find_apply_lem_hyp pointers_in_state_elim.
+      intuition; break_exists; intuition; simpl in *; eauto.
+    + find_apply_lem_hyp pointers_in_state_elim.
+      intuition; break_exists; intuition; simpl in *; eauto.
+      * repeat (handler_def || handler_simpl);
+          try solve [assert (In p (succ_list st)) by (repeat find_rewrite; in_crush); eauto].
+      * repeat (handler_def || handler_simpl).
+        admit (* need to add timeouts *).
+      * repeat (handler_def || handler_simpl).
+      * repeat (handler_def || handler_simpl);
+          try solve [find_apply_lem_hyp option_map_Some; break_exists;
+                     intuition; repeat find_inversion; eauto; subst; simpl in *; intuition];
+          try solve [in_crush; eauto; unfold send_keepalives in *; in_crush].
+    + find_apply_lem_hyp pointers_in_state_elim.
+      intuition; break_exists; intuition; simpl in *; eauto.
+      * repeat (handler_def || (try find_apply_lem_hyp in_make_succs; intuition) || handler_simpl);
+          try solve [assert (In p (succ_list st)) by (repeat find_rewrite; in_crush); eauto];
+          try solve [
+                repeat find_rewrite; 
+                in_crush; eauto;
+                apply H2;
+                eapply in_network_in_pointers_in_state with (m := m); eauto;
+                repeat find_rewrite; in_crush].
+        -- 
+Admitted.
+        
+      
+        (*
+Theorem big_joined_invariant :
+  forall gst,
+    reachable_st gst ->
+    all_payload_pointers_joined gst /\
+    succs_joined gst /\
+    pred_joined gst.
+Proof.
+  intros.
+  induction H.
+  - intuition.
+    + unfold initial_st in *.
+      unfold all_payload_pointers_joined. intuition.
+      repeat find_rewrite. in_crush.
+    + unfold succs_joined. intuition.
+      find_copy_eapply_lem_hyp sigma_some_in_nodes; try solve [constructor; auto].
+      find_copy_apply_lem_hyp sigma_initial_st_start_handler; auto.
+      subst. unfold start_handler in *.
+      repeat break_match; simpl in *; intuition.
+      cut (In (addr_of p) (nodes gst)).
+      { intros. find_apply_lem_hyp initial_nodes_live; eauto.
+        unfold live_node in *. intuition.
+      }
+      cut (In p (sort_by_between h (map make_pointer (nodes gst)))).
+      {
+        intros.
+        find_apply_lem_hyp in_sort_by_between.
+        in_crush.
+      }
+      repeat find_rewrite.
+      find_apply_lem_hyp in_firstn.
+      in_crush.
+    + unfold pred_joined. intuition.
+      find_copy_eapply_lem_hyp sigma_some_in_nodes; try solve [constructor; auto].
+      find_copy_apply_lem_hyp sigma_initial_st_start_handler; auto.
+      subst. unfold start_handler in *.
+      repeat break_match; simpl in *; intuition; try congruence.
+      cut (In (addr_of p) (nodes gst)).
+      { intros. find_apply_lem_hyp initial_nodes_live; eauto.
+        unfold live_node in *. intuition.
+      }
+      cut (In p (sort_by_between h (map make_pointer (nodes gst)))).
+      {
+        intros.
+        find_apply_lem_hyp in_sort_by_between.
+        in_crush.
+      }
+      repeat find_rewrite.
+      eauto using find_pred_in.
+  - inv_prop step_dynamic; simpl in *; eauto.
+    + intuition.
+      * unfold all_payload_pointers_joined. simpl.
+        intros. intuition; subst; simpl in *; intuition.
+        update_destruct; subst; rewrite_update; eauto.
+        exfalso.
+        eapply_prop_hyp all_payload_pointers_joined pointers_in_payload; auto.
+        break_exists. intuition.
+        find_eapply_lem_hyp sigma_some_in_nodes; eauto.
+      * unfold succs_joined. simpl. intuition.
+        repeat (update_destruct; subst; rewrite_update; eauto).
+        -- find_inversion. simpl in *. intuition.
+        -- exfalso.
+           eapply_prop_hyp succs_joined succ_list; eauto.
+           break_exists. intuition.
+           find_eapply_lem_hyp sigma_some_in_nodes; eauto.
+        -- exfalso. find_inversion. simpl in *. intuition.
+      * unfold pred_joined. simpl. intuition.
+        repeat (update_destruct; subst; rewrite_update; eauto).
+        -- find_inversion. simpl in *. congruence.
+        -- exfalso.
+           eapply_prop_hyp pred_joined pred; eauto.
+           break_exists. intuition.
+           find_eapply_lem_hyp sigma_some_in_nodes; eauto.
+        -- exfalso. find_inversion. simpl in *. congruence.
+    + intuition.
+      * unfold all_payload_pointers_joined. intuition.
+        simpl in *.
+        repeat (handler_def || (handler_simpl; in_crush));
+          try find_apply_lem_hyp option_map_Some;
+          try solve
+              [intuition; eauto;
+               break_exists; intuition; find_inversion; simpl in *; intuition];
+          try solve [unfold send_keepalives in *; in_crush];
+          try solve [
+                eapply_prop_hyp all_payload_pointers_joined pointers_in_payload; eauto;
+                repeat find_rewrite; break_exists; intuition; repeat find_inversion; eauto].
+      * unfold succs_joined. intuition. simpl in *.
+        repeat (handler_def || (handler_simpl; in_crush));
+          try find_apply_lem_hyp option_map_Some;
+          try assert (In p (succ_list st)) by (repeat find_rewrite; in_crush);
+          try solve [
+                eapply_prop_hyp succs_joined succ_list; eauto;
+                repeat find_rewrite; eauto; break_exists; intuition; repeat find_inversion; eauto].
+      * unfold pred_joined. intuition. simpl in *.
+        repeat (handler_def || (handler_simpl; in_crush));
+          try find_apply_lem_hyp option_map_Some;
+          try solve [
+                eapply_prop_hyp pred_joined pred; eauto;
+                repeat find_rewrite; eauto; break_exists; intuition; repeat find_inversion; eauto].
+        assert (In p (succ_list st)) by (repeat find_rewrite; in_crush).
+        -- eapply_prop_hyp succs_joined succ_list; eauto.
+           repeat find_rewrite; eauto; break_exists; intuition; repeat find_inversion; eauto.
+        -- eapply_prop_hyp all_payload_pointers_joined pointers_in_payload; eauto.
+           repeat find_rewrite. break_exists. intuition; repeat find_inversion; eauto.
+           eexists; intuition; simpl; eauto.
+        eauto.
+        eexists; intuition; eauto.
+        eauto.
+        eexists; intuition; eauto. simpl.
+        eapply_prop_hyp all_payload_pointers_joined msgs; eauto.
+        
+        -- unfold send_keepalives in *. in_crush.
+        
+        -- eapply_prop all_payload_pointers_joined; eauto. in_crush.
+*)        
+(*
+Theorem big_joined_invariant :
+  forall gst,
+    reachable_st gst ->
+    all_payload_pointers_joined gst /\
+    succs_joined gst.
+Proof.
+  intros.
+  induction H.
+  - intuition.
+    + unfold initial_st in *.
+      unfold all_payload_pointers_joined. intuition.
+      repeat find_rewrite. in_crush.
+    + unfold succs_joined. intuition.
+      find_copy_eapply_lem_hyp sigma_some_in_nodes; try solve [constructor; auto].
+      find_copy_apply_lem_hyp sigma_initial_st_start_handler; auto.
+      subst. unfold start_handler in *.
+      repeat break_match; simpl in *; intuition.
+      cut (In (addr_of p) (nodes gst)).
+      { intros. find_apply_lem_hyp initial_nodes_live; eauto.
+        unfold live_node in *. intuition.
+      }
+      cut (In p (sort_by_between h (map make_pointer (nodes gst)))).
+      {
+        intros.
+        find_apply_lem_hyp in_sort_by_between.
+        in_crush.
+      }
+      repeat find_rewrite.
+      find_apply_lem_hyp in_firstn.
+      in_crush.
+  - inv_prop step_dynamic; simpl in *; eauto.
+    + intuition.
+      * unfold all_payload_pointers_joined. simpl.
+        intros. intuition; subst; simpl in *; intuition.
+        update_destruct; subst; rewrite_update; eauto.
+        exfalso.
+        eapply_prop_hyp all_payload_pointers_joined pointers_in_payload; auto.
+        break_exists. intuition.
+        find_eapply_lem_hyp sigma_some_in_nodes; eauto.
+      * unfold succs_joined. simpl. intuition.
+        repeat (update_destruct; subst; rewrite_update; eauto).
+        -- find_inversion. simpl in *. intuition.
+        -- exfalso.
+           eapply_prop_hyp succs_joined succ_list; eauto.
+           break_exists. intuition.
+           find_eapply_lem_hyp sigma_some_in_nodes; eauto.
+        -- exfalso. find_inversion. simpl in *. intuition.
+    + intuition.
+      * unfold all_payload_pointers_joined. intuition.
+        simpl in *.
+        repeat (handler_def || (handler_simpl; in_crush));
+          try find_apply_lem_hyp option_map_Some;
+          try solve
+              [intuition; eauto;
+               break_exists; intuition; find_inversion; simpl in *; intuition];
+          try solve [unfold send_keepalives in *; in_crush];
+          try solve [
+                eapply_prop_hyp all_payload_pointers_joined pointers_in_payload; eauto;
+                repeat find_rewrite; break_exists; intuition; repeat find_inversion; eauto].
+      * unfold succs_joined. intuition. simpl in *.
+        repeat (handler_def || (handler_simpl; in_crush));
+          try find_apply_lem_hyp option_map_Some;
+          try assert (In p (succ_list st)) by (repeat find_rewrite; in_crush);
+          try solve [
+                eapply_prop_hyp succs_joined succ_list; eauto;
+                repeat find_rewrite; eauto; break_exists; intuition; repeat find_inversion; eauto].
+    + intuition.
+      * unfold all_payload_pointers_joined. intuition. simpl in *.
+        repeat (handler_def || (handler_simpl; in_crush)).
+*)      
 Theorem stabilize_target_joined :
   forall gst h st dst m,
     reachable_st gst ->
